WIP

src/ModSimStutter.v
@@ -44,16 +44,16 @@ Section PRIMIVIESIM.
 
   Variant __lsim
           (tid: thread_id)
-          (lsim: forall R_src R_tgt (RR: R_src -> R_tgt -> URA.car -> shared_rel), bool -> bool -> URA.car -> (wf_stt.(T) * itree srcE R_src) -> itree tgtE R_tgt -> shared_rel)
-          (_lsim: forall R_src R_tgt (RR: R_src -> R_tgt -> URA.car -> shared_rel),bool -> bool -> URA.car -> (wf_stt.(T) * itree srcE R_src) -> itree tgtE R_tgt -> shared_rel)
-          R_src R_tgt (RR: R_src -> R_tgt -> URA.car -> shared_rel)
+          (lsim: forall R_src R_tgt (RR: R_src -> R_tgt -> URA.car -> wf_stt.(T) -> shared_rel), bool -> bool -> URA.car -> (wf_stt.(T) * itree srcE R_src) -> itree tgtE R_tgt -> shared_rel)
+          (_lsim: forall R_src R_tgt (RR: R_src -> R_tgt -> URA.car -> wf_stt.(T) -> shared_rel),bool -> bool -> URA.car -> (wf_stt.(T) * itree srcE R_src) -> itree tgtE R_tgt -> shared_rel)
+          R_src R_tgt (RR: R_src -> R_tgt -> URA.car -> wf_stt.(T) -> shared_rel)
     :
     bool -> bool -> URA.car -> (wf_stt.(T) * itree srcE R_src) -> itree tgtE R_tgt -> shared_rel :=
   | lsim_ret
       f_src f_tgt r_ctx o
       ths im_src im_tgt st_src st_tgt r_shared
       r_src r_tgt
-      (LSIM: RR r_src r_tgt r_ctx (ths, im_src, im_tgt, st_src, st_tgt, r_shared))
+      (LSIM: RR r_src r_tgt r_ctx o (ths, im_src, im_tgt, st_src, st_tgt, r_shared))
     :
     __lsim tid lsim _lsim RR f_src f_tgt r_ctx (o, Ret r_src) (Ret r_tgt) (ths, im_src, im_tgt, st_src, st_tgt, r_shared)
 
@@ -199,7 +199,7 @@ Section PRIMIVIESIM.
   .
 
   Definition lsim (tid: thread_id)
-             R_src R_tgt (RR: R_src -> R_tgt -> URA.car -> shared_rel):
+             R_src R_tgt (RR: R_src -> R_tgt -> URA.car -> wf_stt.(T) -> shared_rel):
     bool -> bool -> URA.car -> (wf_stt.(T) * itree srcE R_src) -> itree tgtE R_tgt -> shared_rel :=
     paco9 (fun r => pind9 (__lsim tid r) top9) bot9 R_src R_tgt RR.
 
@@ -226,8 +226,8 @@ Section PRIMIVIESIM.
   Qed.
 
   Variant lsim_resetC
-          (r: forall R_src R_tgt (RR: R_src -> R_tgt -> URA.car -> shared_rel), bool -> bool -> URA.car -> (wf_stt.(T) * itree srcE R_src) -> itree tgtE R_tgt -> shared_rel)
-          R_src R_tgt (RR: R_src -> R_tgt -> URA.car -> shared_rel)
+          (r: forall R_src R_tgt (RR: R_src -> R_tgt -> URA.car -> wf_stt.(T) -> shared_rel), bool -> bool -> URA.car -> (wf_stt.(T) * itree srcE R_src) -> itree tgtE R_tgt -> shared_rel)
+          R_src R_tgt (RR: R_src -> R_tgt -> URA.car -> wf_stt.(T) -> shared_rel)
     :
     bool -> bool -> URA.car -> (wf_stt.(T) * itree srcE R_src) -> itree tgtE R_tgt -> shared_rel :=
     | lsim_resetC_intro
@@ -250,7 +250,7 @@ Section PRIMIVIESIM.
     { ii. inv IN. econs; eauto. }
     i. inv PR. eapply GF in REL.
     eapply pind9_acc in REL.
-    instantiate (1:= (fun R0 R1 (RR: R0 -> R1 -> URA.car -> shared_rel) ps1 pt1 r_ctx src tgt shr =>
+    instantiate (1:= (fun R0 R1 (RR: R0 -> R1 -> URA.car -> wf_stt.(T) -> shared_rel) ps1 pt1 r_ctx src tgt shr =>
                         forall ps0 pt0,
                           (ps1 = true -> ps0 = true) ->
                           (pt1 = true -> pt0 = true) ->
@@ -330,7 +330,7 @@ Section PRIMIVIESIM.
 
   Lemma lsim_reset_prog
         tid
-        R0 R1 (RR: R0 -> R1 -> URA.car -> shared_rel)
+        R0 R1 (RR: R0 -> R1 -> URA.car -> wf_stt.(T) -> shared_rel)
         src tgt shr
         ps0 pt0 ps1 pt1 r_ctx
         (LSIM: lsim tid RR ps1 pt1 r_ctx src tgt shr)
@@ -351,7 +351,7 @@ Section PRIMIVIESIM.
 
   Lemma lsim_set_prog
         tid
-        R0 R1 (RR: R0 -> R1 -> URA.car -> shared_rel)
+        R0 R1 (RR: R0 -> R1 -> URA.car -> wf_stt.(T) -> shared_rel)
         r_ctx src tgt shr
         (LSIM: lsim tid RR true true r_ctx src tgt shr)
     :
@@ -363,7 +363,7 @@ Section PRIMIVIESIM.
     2:{ eapply lsim_mon. }
     eapply pind9_acc in LSIM.
 
-    { instantiate (1:= (fun R0 R1 (RR: R0 -> R1 -> URA.car -> shared_rel) ps0 pt0 r_ctx src tgt shr =>
+    { instantiate (1:= (fun R0 R1 (RR: R0 -> R1 -> URA.car -> wf_stt.(T) -> shared_rel) ps0 pt0 r_ctx src tgt shr =>
                           ps0 = true ->
                           pt0 = true ->
                           forall ps pt,
@@ -448,38 +448,44 @@ Section PRIMIVIESIM.
   Qed.
 
   Definition local_RR {R0 R1} (RR: R0 -> R1 -> Prop) tid:
-    R0 -> R1 -> URA.car -> shared_rel :=
-    fun (r_src: R0) (r_tgt: R1) (r_ctx: URA.car) '(ths2, im_src1, im_tgt1, st_src1, st_tgt1, r_shared1) =>
-      (exists ths3 r_own r_shared2,
+    R0 -> R1 -> URA.car -> wf_stt.(T) -> shared_rel :=
+    fun (r_src: R0) (r_tgt: R1) (r_ctx: URA.car) (o: wf_stt.(T)) '(ths2, im_src1, im_tgt1, st_src1, st_tgt1, r_shared1) =>
+      (exists ths3 r_own o0 r_shared2,
           (<<THS: NatMap.remove tid ths2 = ths3>>) /\
             (<<VALID: URA.wf (r_shared2 ⋅ r_own ⋅ r_ctx)>>) /\
             (<<INV: I (ths3, im_src1, im_tgt1, st_src1, st_tgt1, r_shared2)>>) /\
+            (<<STT: wf_stt.(lt) o0 o>>) /\
             (<<RET: RR r_src r_tgt>>)).
+
+  Definition embed_lrr {R0 R1} (LRR: R0 -> R1 -> URA.car -> shared_rel):
+    R0 -> R1 -> URA.car -> wf_stt.(T) -> shared_rel :=
+    fun (r_src: R0) (r_tgt: R1) (r_ctx: URA.car) (o: wf_stt.(T)) shr =>
+      (<<LSIM: LRR r_src r_tgt r_ctx shr>>) /\ (<<STT: exists o0, wf_stt.(lt) o0 o>>).
 
   Definition local_sim {R0 R1} (RR: R0 -> R1 -> Prop) src tgt :=
     forall ths0 im_src0 im_tgt0 st_src0 st_tgt0 r_shared0 r_ctx0
-           (INV: I (ths0, im_src0, im_tgt0, st_src0, st_tgt0, r_shared0))
-           tid ths1
-           (THS: TIdSet.add_new tid ths0 ths1)
-           (VALID: URA.wf (r_shared0 ⋅ r_ctx0)),
+      (INV: I (ths0, im_src0, im_tgt0, st_src0, st_tgt0, r_shared0))
+      tid ths1
+      (THS: TIdSet.add_new tid ths0 ths1)
+      (VALID: URA.wf (r_shared0 ⋅ r_ctx0)),
     exists r_shared1 r_own,
       (<<INV: I (ths1, im_src0, im_tgt0, st_src0, st_tgt0, r_shared1)>>) /\
         (<<VALID: URA.wf (r_shared1 ⋅ r_own ⋅ r_ctx0)>>) /\
         (forall ths im_src1 im_tgt1 st_src st_tgt r_shared2 r_ctx2
-                (INV: I (ths, im_src1, im_tgt1, st_src, st_tgt, r_shared2))
-                (VALID: URA.wf (r_shared2 ⋅ r_own ⋅ r_ctx2)),
+           (INV: I (ths, im_src1, im_tgt1, st_src, st_tgt, r_shared2))
+           (VALID: URA.wf (r_shared2 ⋅ r_own ⋅ r_ctx2)),
           forall im_tgt2 (TGT: fair_update im_tgt1 im_tgt2 (sum_fmap_l (tids_fmap tid ths))),
-          exists im_src2 o,
-            (<<SRC: fair_update im_src1 im_src2 (sum_fmap_l (tids_fmap tid ths))>>) /\
-              (<<LSIM: forall fs ft,
-                  lsim
-                    tid
-                    (@local_RR R0 R1 RR tid)
-                    fs ft
-                    r_ctx2
-                    (o, src) tgt
-                    (ths, im_src2, im_tgt2, st_src, st_tgt, r_shared2)
-                    >>)).
+          exists o,
+          exists im_src2, (<<SRC: fair_update im_src1 im_src2 (sum_fmap_l (tids_fmap tid ths))>>) /\
+                       (<<LSIM: forall fs ft,
+                           lsim
+                             tid
+                             (@local_RR R0 R1 RR tid)
+                             fs ft
+                             r_ctx2
+                             (o, src) tgt
+                             (ths, im_src2, im_tgt2, st_src, st_tgt, r_shared2)
+                             >>)).
 
   Definition shared_rel_wf: Prop :=
     forall ths im_src0 im_tgt0 st_src st_tgt r_shared0 r_ctx
